Refactor to allow proofs about BB(3, 3)

verify/Extraction.v
@@ -1,48 +1,14 @@
 (** * Extraction to OCaml *)
 
 From Coq Require Extraction.
-From Coq Require Import Lists.List. Import ListNotations.
 Require Import ExtrOcamlBasic.
 Require Import ExtrOcamlIntConv.
-From BusyCoq Require Export Cyclers TranslatedCyclers BackwardsReasoning Bouncers.
+From BusyCoq Require Export BB52 Cyclers TranslatedCyclers BackwardsReasoning Bouncers.
 
-Inductive state := A | B | C | D | E.
-Inductive sym := S0 | S1.
-
-Module Ctx <: Ctx.
-  Definition Q := state.
-  Definition Sym := sym.
-  Definition q0 := A.
-  Definition s0 := S0.
-
-  Definition eqb_q (a b : Q): {a = b} + {a <> b}.
-    decide equality.
-  Defined.
-
-  Definition eqb_sym (a b : Sym): {a = b} + {a <> b}.
-    decide equality.
-  Defined.
-
-  Definition all_qs := [A; B; C; D; E].
-
-  Lemma all_qs_spec : forall a, In a all_qs.
-  Proof.
-    destruct a; repeat ((left; reflexivity) || right).
-  Qed.
-
-  Definition all_syms := [S0; S1].
-
-  Lemma all_syms_spec : forall a, In a all_syms.
-  Proof.
-    destruct a; repeat ((left; reflexivity) || right).
-  Qed.
-End Ctx.
-
-Module EFlip := Flip Ctx.
-Module ECyclers := Cyclers Ctx.
-Module ETranslatedCyclers := TranslatedCyclers Ctx.
-Module EBackwardsReasoning := BackwardsReasoning Ctx.
-Module EBouncers := Bouncers Ctx.
+Module ECyclers := Cyclers BB52.
+Module ETranslatedCyclers := TranslatedCyclers BB52.
+Module EBackwardsReasoning := BackwardsReasoning BB52.
+Module EBouncers := Bouncers BB52.
 
 Extraction Language OCaml.
 Extraction "extraction.ml" nat_of_int
