verify/BB33.v
@@ -1,0 +1,37 @@
+(** * Instantiating the development to machines with 3 states and 3 symbols *)
+
+From Coq Require Import Lists.List. Import ListNotations.
+From BusyCoq Require Export Flip.
+Set Default Goal Selector "!".
+
+Inductive state := A | B | C.
+Inductive sym := S0 | S1 | S2.
+
+Module BB33 <: Ctx.
+  Definition Q := state.
+  Definition Sym := sym.
+  Definition q0 := A.
+  Definition s0 := S0.
+
+  Definition eqb_q (a b : Q): {a = b} + {a <> b}.
+    decide equality.
+  Defined.
+
+  Definition eqb_sym (a b : Sym): {a = b} + {a <> b}.
+    decide equality.
+  Defined.
+
+  Definition all_qs := [A; B; C].
+
+  Lemma all_qs_spec : forall a, In a all_qs.
+  Proof.
+    destruct a; repeat ((left; reflexivity) || right).
+  Qed.
+
+  Definition all_syms := [S0; S1; S2].
+
+  Lemma all_syms_spec : forall a, In a all_syms.
+  Proof.
+    destruct a; repeat ((left; reflexivity) || right).
+  Qed.
+End BB33.
