verify/Individual33.v
@@ -1,0 +1,7 @@
+From BusyCoq Require Export Individual BB33.
+
+Module Individual33 := Individual BB33.
+
+Notation "0" := S0.
+Notation "1" := S1.
+Notation "2" := S2.
