verify/Individual52.v
@@ -1,0 +1,6 @@
+From BusyCoq Require Export Individual BB52.
+
+Module Individual52 := Individual BB52.
+
+Notation "0" := S0.
+Notation "1" := S1.
